WIP: simrel_cert_step lemmas

Coq/src/SimRelCertStep.v
@@ -117,7 +117,7 @@ Section SimRelCertStep.
   Notation "'cont_lang'" :=
     (fun S k => thread_lts (ES.cont_thread S k)) (at level 10, only parsing).
 
-  Definition cert_step_fence
+  Definition cert_fence_step
              (e  : eventid)
              (e' : option eventid)
              (S S' : ES.t) : Prop :=
@@ -127,7 +127,7 @@ Section SimRelCertStep.
     ⟪ EW' : Sew S' ≡ Sew S ⟫ /\
     ⟪ CO' : Sco S' ≡ Sco S ⟫.
 
-  Definition cert_step_load
+  Definition cert_load_step
              (thread : thread_id)
              (st : thread_st thread)
              (e : eventid)
@@ -139,7 +139,7 @@ Section SimRelCertStep.
       ⟪ EW' : Sew S' ≡ Sew S ⟫ /\
       ⟪ CO' : Sco S' ≡ Sco S ⟫.
 
-  Definition cert_step_store
+  Definition cert_store_step
              (thread : thread_id)
              (st : thread_st thread)
              (e  : eventid)
@@ -151,7 +151,7 @@ Section SimRelCertStep.
       ⟪ AEW : sim_add_ew TC f ews e S S' ⟫ /\
       ⟪ ACO : sim_add_co G e S S' ⟫.
 
-  Definition cert_step_update
+  Definition cert_update_step
              (thread : thread_id)
              (st : thread_st thread)
              (e  : eventid)
@@ -169,10 +169,10 @@ Section SimRelCertStep.
              (e  : eventid)
              (e' : option eventid)
              (S S' : ES.t) : Prop := 
-    cert_step_fence e e' S S' \/ 
-    cert_step_load  st e e' S S' \/ 
-    cert_step_store st e e' S S' \/ 
-    cert_step_update st e e' S S'. 
+    cert_fence_step e e' S S' \/ 
+    cert_load_step  st e e' S S' \/ 
+    cert_store_step st e e' S S' \/ 
+    cert_update_step st e e' S S'. 
 
   Definition cert_step 
              (e  : eventid)
@@ -184,7 +184,7 @@ Section SimRelCertStep.
 
   Ltac unfold_cert_step H := 
     unfold cert_step, cert_step_, 
-           cert_step_fence, cert_step_load, cert_step_store, cert_step_update 
+           cert_fence_step, cert_load_step, cert_store_step, cert_update_step 
       in H; destruct H as [HA | [HB | [HC | HD]]]; desc.
 
 Section SimRelCertStepProps. 
@@ -238,6 +238,240 @@ Section SimRelCertStepProps.
     (*     by rewrite inter_false_l. }  *)
     (* all: basic_solver. *)
   Admitted.
+
+  Lemma simrel_cert_basic_step k lbl lbl' lbls S jf ew co
+        (st st' st'' : thread_st (ES.cont_thread S k))
+        (SRCC : simrel_cert prog S G sc TC f TC' h k st st'') 
+        (ILBL_STEP : ilbl_step (ES.cont_thread S k) lbls st st') 
+        (LBLS_EQ : lbls = opt_to_list lbl' ++ [lbl]) :
+    exists k' e e' S',
+      ⟪ BSTEP_ : ESBasicStep.t_ (thread_lts (ES.cont_thread S k)) k k' st st' e e' S S' ⟫ /\
+      ⟪ LBL  : lbl  = S'.(ES.lab) e ⟫ /\
+      ⟪ LBL' : lbl' = option_map S'.(ES.lab) e' ⟫ /\
+      ⟪ JF' : S'.(ES.jf) ≡ jf ⟫ /\
+      ⟪ EW' : S'.(ES.ew) ≡ ew ⟫ /\
+      ⟪ CO' : S'.(ES.co) ≡ co ⟫.
+  Proof.
+    assert (tc_coherent G sc TC') as TCCOH'. 
+    { eapply isim_trav_step_coherence; apply SRCC. }
+    assert ((K S) (k, existT Language.state (thread_lts (ES.cont_thread S k)) st)) as KK.
+    { edestruct cstate_q_cont; [apply SRCC|]. desf. }
+    assert (wf_thread_state (ES.cont_thread S k) st) as WFST.
+    { by apply SRCC. }
+
+    set (ILBL_STEP' := ILBL_STEP).
+    eapply lbl_step_cases in ILBL_STEP'; auto. 
+    subst lbls. desc.
+    eapply opt_to_list_app_singl in LBLS. 
+    desf.
+
+    1-4 : 
+      exists (CEvent S.(ES.next_act)); 
+      exists S.(ES.next_act); exists None;
+      eexists (ES.mk _ _ _ _ _ _ _ _ _);
+      splits; simpl; eauto;
+      [ econstructor; splits; simpl; eauto; 
+        eexists; exists None; 
+        splits; simpl; eauto; 
+        eapply ILBL_STEP 
+      | by rewrite upds ].
+
+    exists (CEvent (1 + S.(ES.next_act))). 
+    exists S.(ES.next_act). exists (Some (1 + S.(ES.next_act))).
+    eexists (ES.mk _ _ _ _ _ _ _ _ _).
+    econstructor; splits; simpl; eauto. 
+    { econstructor; splits; simpl; eauto. 
+      eexists; eexists. 
+      splits; simpl; eauto; by simpl. }
+    { rewrite updo; [|omega]. by rewrite upds. }
+    by rewrite upds.
+  Qed.
+
+  (* Lemma simrel_cert_basic_step_cert_rf k k' e e' S S'  *)
+  (*       (st st' st'' : thread_st (ES.cont_thread S k)) *)
+  (*       (SRCC : simrel_cert prog S G sc TC f TC' h k st st'')  *)
+  (*       (BSTEP_ : ESBasicStep.t_ (thread_lts (ES.cont_thread S k)) k k' st st' e e' S S')  *)
+  (*       (CST_REACHABLE : (lbl_step (ES.cont_thread S k))＊ st' st'') *)
+  (*       (RR : exists is_ex ord loc val, ⟪ LBL_LD : Slab S' e = Aload is_ex ord loc val ⟫) : *)
+  (*   exists w,  *)
+  (*     ⟪hCertDOMw : (h □₁ cert_dom G TC (ES.cont_thread S k) st) w⟫ /\ *)
+  (*     ⟪CertRF : cert_rf G sc TC' (ES.cont_thread S k) (e2a S' w) (e2a S' e)⟫. *)
+  (* Proof.  *)
+  (*   cdes BSTEP_. *)
+  (*   assert (ESBasicStep.t e e' S S') as BSTEP. *)
+  (*   { econstructor. eauto. } *)
+  (*   assert (ES.Wf S) as WF. *)
+  (*   { apply SRCC. } *)
+  (*   assert (tc_coherent G sc TC') as TCCOH'.  *)
+  (*   { eapply isim_trav_step_coherence; apply SRCC. } *)
+  (*   assert ((K S) (k, existT Language.state (thread_lts (ES.cont_thread S k)) st)) as KK. *)
+  (*   { edestruct cstate_q_cont; [apply SRCC|]. desf. } *)
+  (*   assert (wf_thread_state (ES.cont_thread S k) st) as WFST. *)
+  (*   { by apply SRCC. } *)
+  (*   assert (lbl = Aload is_ex ord loc val) as LBL_EQ. *)
+  (*   { rewrite <- LBL_LD, LAB'. *)
+  (*     rewrite updo_opt, upds; auto. *)
+  (*     ESBasicStep.step_solver. } *)
+  (*   edestruct cert_rf_complete as [w RFwa];  *)
+  (*     eauto; try apply SRCC. *)
+  (*   { assert  *)
+  (*       (E0 G TC' (ES.cont_thread S k) (ThreadEvent (ES.cont_thread S k) st.(eindex))) *)
+  (*       as E0_eindex. *)
+  (*     { eapply ilbl_step_E0_eindex;  *)
+  (*         eauto; [apply SRCC | apply STEP]. } *)
+  (*     split; eauto. *)
+  (*     eapply same_lab_u2v_dom_is_r. *)
+  (*     { apply same_lab_u2v_dom_comm. *)
+  (*       eapply cuplab_cert. apply SRCC. } *)
+  (*     split.  *)
+  (*     { eapply dcertE; eauto; apply SRCC. } *)
+  (*     unfold is_r. *)
+  (*     erewrite steps_preserve_lab. *)
+  (*     { edestruct lbl_step_cases as [la [lb [LBLS HH]]]; eauto. *)
+  (*       { apply STEP. } *)
+  (*       apply opt_to_list_app_singl in LBLS. *)
+  (*       desc. subst la lb. *)
+  (*       destruct HH as [HA | HB]. *)
+  (*       { destruct HA as [_ [_ [LAB _]]]. *)
+  (*         rewrite LAB, upds. desf. } *)
+  (*       destruct HB as [_ [_ [LAB [LBLS' RMW]]]]. *)
+  (*       rewrite LAB.  *)
+  (*       rewrite updo_opt, upds; desf. *)
+  (*       red. ins. inv H. omega. } *)
+  (*     { eapply wf_thread_state_steps; eauto. *)
+  (*       eapply ilbl_steps_in_steps. *)
+  (*       econstructor; econstructor; eauto.  *)
+  (*       apply STEP. } *)
+  (*     { by eapply ilbl_steps_in_steps. } *)
+  (*     edestruct lbl_step_cases as [la [lb [LBLS HH]]]; eauto. *)
+  (*     { apply STEP. } *)
+  (*     generalize HH. basic_solver. } *)
+    
+  (*   assert (cert_dom G TC (ES.cont_thread S k) st w) as HDOMw. *)
+  (*   { eapply cert_rf_cert_dom; try apply SRCC; auto.  *)
+  (*     { red. ins. eapply ES.init_tid_K; eauto. } *)
+  (*     unfold dom_rel. eexists. *)
+  (*     apply seq_eqv_r; splits; eauto. } *)
+  (*   assert  *)
+  (*     ((h □₁ (cert_dom G TC (ES.cont_thread S k) st)) (h w))  *)
+  (*     as hHDOMhw.  *)
+  (*   { unfolder; eexists; splits; eauto. } *)
+    
+  (*   eexists; econstructor; splits; eauto. *)
+  (*   erewrite basic_step_e2a_e with (e := e);  *)
+  (*     eauto; try apply SRCC. *)
+  (*   arewrite (e2a S' (h w) = w); auto. *)
+  (*   erewrite basic_step_e2a_eq_dom; eauto. *)
+  (*   { eapply a2e_fix; eauto. apply SRCC. } *)
+  (*   eapply a2e_img; eauto. apply SRCC.  *)
+  (* Qed. *)
+
+  Lemma simrel_cert_sim_add_jf k lbl lbl' lbls S ew co
+        (st st' st'' : thread_st (ES.cont_thread S k))
+        (SRCC : simrel_cert prog S G sc TC f TC' h k st st'')
+        (ILBL_STEP : ilbl_step (ES.cont_thread S k) lbls st st')
+        (CST_REACHABLE : (lbl_step (ES.cont_thread S k))＊ st' st'')
+        (LBLS_EQ : lbls = opt_to_list lbl' ++ [lbl])
+        (RR : exists is_ex ord loc val, ⟪ LBL_LD : lbl = Aload is_ex ord loc val ⟫) :
+    exists k' w e e' S',
+      ⟪ BSTEP_ : ESBasicStep.t_ (thread_lts (ES.cont_thread S k)) k k' st st' e e' S S' ⟫ /\
+      ⟪ LBL  : lbl  = S'.(ES.lab) e ⟫ /\
+      ⟪ LBL' : lbl' = option_map S'.(ES.lab) e' ⟫ /\
+      ⟪ CAJF : sim_add_jf G sc TC TC' h (ES.cont_thread S k) st w e S S' ⟫ /\
+      ⟪ EW' : S'.(ES.ew) ≡ ew ⟫ /\
+      ⟪ CO' : S'.(ES.co) ≡ co ⟫.
+  Proof.
+    desf.
+    assert (ES.Wf S) as WF.
+    { apply SRCC. }
+    assert (tc_coherent G sc TC') as TCCOH'.
+    { eapply isim_trav_step_coherence; apply SRCC. }
+    assert ((K S) (k, existT Language.state (thread_lts (ES.cont_thread S k)) st)) as KK.
+    { edestruct cstate_q_cont; [apply SRCC|]. desf. }
+    assert (wf_thread_state (ES.cont_thread S k) st) as WFST.
+    { by apply SRCC. }
+    edestruct cert_rf_complete as [w RFwa];
+      eauto; try apply SRCC.
+    { assert
+        (E0 G TC' (ES.cont_thread S k) (ThreadEvent (ES.cont_thread S k) st.(eindex)))
+        as E0_eindex.
+      { eapply ilbl_step_E0_eindex; eauto.
+        all : by eapply SRCC. }
+      split; eauto.
+      eapply same_lab_u2v_dom_is_r.
+      { apply same_lab_u2v_dom_comm.
+        eapply cuplab_cert; apply SRCC. }
+      split.
+      { eapply dcertE; eauto; apply SRCC. }
+      unfold is_r.
+      erewrite steps_preserve_lab.
+      { edestruct lbl_step_cases as [lbl [lbl'' HH]]; eauto.
+        destruct HH as [LBLS [HA | HB]].
+        all : apply opt_to_list_app_singl in LBLS.
+        { destruct HA as [_ [_ [LAB _]]].
+          rewrite LAB, upds. desf. }
+        destruct HB as [_ [_ [LAB LBLS']]].
+        rewrite LAB. unfold upd_opt.
+        destruct lbl'' eqn:Heq.
+        { rewrite updo, upds; desf.
+          intros HH. inversion HH. omega. }
+        exfalso. desf. }
+      { eapply wf_thread_state_steps; eauto.
+        eapply ilbl_steps_in_steps.
+        econstructor; econstructor; eauto. }
+      { by eapply ilbl_steps_in_steps. }
+      edestruct lbl_step_cases as [lbl [lbl'' HH]]; eauto.
+      destruct HH as [LBLS [HH | HH]].
+      all : apply opt_to_list_app_singl in LBLS.
+      all : destruct HH as [_ [ACTS _]].
+      all : apply ACTS; basic_solver. }
+    assert (cert_dom G TC (ES.cont_thread S k) st w) as HDOMw.
+    { eapply cert_rf_cert_dom; try apply SRCC; auto.
+      { red. ins. eapply ES.init_tid_K; eauto. }
+      unfold dom_rel. eexists.
+      apply seq_eqv_r; splits; eauto. }
+    assert
+      ((h □₁ (cert_dom G TC (ES.cont_thread S k) st)) (h w))
+      as hHDOMhw.
+    { unfolder; eexists; splits; eauto. }
+
+    edestruct simrel_cert_basic_step as [k' [e [e' [S' HH]]]]; eauto.
+    desf; do 5 eexists; splits; eauto.
+    assert (ESBasicStep.t e e' S S') as BSTEP.
+    { econstructor. eauto. }
+    econstructor; splits; eauto.
+    { eapply ESBasicStep.basic_step_acts_set; eauto. basic_solver. }
+    { unfold is_r. by rewrite <- LBL. }
+    { erewrite basic_step_e2a_e with (e := e);
+        eauto; try apply SRCC.
+      arewrite (e2a S' (h w) = w); auto.
+      erewrite basic_step_e2a_eq_dom.
+      { eapply a2e_fix; eauto. apply SRCC. }
+      { apply SRCC. }
+      { econstructor; eauto. }
+      eapply a2e_img; eauto. apply SRCC. }
+    cdes BSTEP_. rewrite EVENT. apply JF'.
+  Qed.
+
+  Lemma simrel_cert_load_step k lbl S
+        (st st' st'' : thread_st (ES.cont_thread S k))
+        (SRCC : simrel_cert prog S G sc TC f TC' h k st st'') 
+        (ILBL_STEP : ilbl_step (ES.cont_thread S k) [lbl] st st') 
+        (CST_REACHABLE : (lbl_step (ES.cont_thread S k))＊ st' st'')
+        (RR : exists is_ex ord loc val, ⟪ LBL_LD : lbl = Aload is_ex ord loc val ⟫) :
+    exists k' e e' S', 
+      ⟪ BSTEP_ : ESBasicStep.t_ (thread_lts (ES.cont_thread S k)) k k' st st' e e' S S' ⟫ /\
+      ⟪ CertLSTEP  : cert_load_step st e e' S S' ⟫ /\
+      ⟪ LBL  : lbl = S'.(ES.lab) e ⟫.
+  Proof. 
+    edestruct simrel_cert_sim_add_jf as [k' [ w [e [e' [S' HH]]]]]; eauto.
+    { erewrite opt_to_list_none. done. }    
+    desf.
+    do 4 eexists; splits; eauto.
+    econstructor; splits; eauto.
+    unfold option_map in LBL'.
+    destruct e'; done. 
+  Qed.
 
   Lemma simrel_cert_step_step_ k k' e e' S S'
         (st st' st'' : thread_st (ES.cont_thread S k))
@@ -642,129 +876,7 @@ Section SimRelCertStepProps.
     unfold eq_opt. basic_solver 5.
   Qed.
 
-  Lemma simrel_cert_basic_step k lbl lbl' lbls jf ew co
-        (st st': (thread_lts (ES.cont_thread S k)).(Language.state))
-        (WFTS : wf_thread_state (ES.cont_thread S k) st)
-        (KK : K S (k, existT _ _ st))
-        (ILBL_STEP : ilbl_step (ES.cont_thread S k) lbls st st') 
-        (LBLS_EQ : lbls = opt_to_list lbl' ++ [lbl]) :
-    exists k' e e' S',
-      ⟪ ES_BSTEP_ : ESBasicStep.t_ (thread_lts (ES.cont_thread S k)) k k' st st' e e' S S' ⟫ /\
-      ⟪ LBL  : lbl  = S'.(ES.lab) e ⟫ /\
-      ⟪ LBL' : lbl' = option_map S'.(ES.lab) e' ⟫ /\
-      ⟪ JF' : S'.(ES.jf) ≡ jf ⟫ /\
-      ⟪ EW' : S'.(ES.ew) ≡ ew ⟫ /\
-      ⟪ CO' : S'.(ES.co) ≡ co ⟫.
-  Proof.
-    set (ILBL_STEP' := ILBL_STEP).
-    eapply lbl_step_cases in ILBL_STEP'; auto.  
-    desf. 
 
-    all : eapply opt_to_list_app_singl in LBLS; desf.
-
-    1-4 : 
-      exists (CEvent S.(ES.next_act)); 
-      exists S.(ES.next_act); exists None;
-      eexists (ES.mk _ _ _ _ _ _ _ _ _);
-      splits; simpl; eauto;
-      [ econstructor; splits; simpl; eauto; 
-        eexists; exists None; 
-        splits; simpl; eauto; 
-        eapply ILBL_STEP 
-      | by rewrite upds ].
-
-    exists (CEvent (1 + S.(ES.next_act))). 
-    exists S.(ES.next_act). exists (Some (1 + S.(ES.next_act))).
-    eexists (ES.mk _ _ _ _ _ _ _ _ _).
-    econstructor; splits; simpl; eauto. 
-    { econstructor; splits; simpl; eauto. 
-      eexists; eexists. 
-      splits; simpl; eauto; by simpl. }
-    { rewrite updo; [|omega]. by rewrite upds. }
-    by rewrite upds.
-  Qed.
-
-  Lemma simrel_cert_add_jf TC' h k lbl lbl' lbls ew co
-        (st st' st'' : thread_st (ES.cont_thread S k))
-        (SRCC : simrel_cert prog S G sc TC f TC' h k st st'') 
-        (ILBL_STEP : ilbl_step (ES.cont_thread S k) lbls st st') 
-        (CST_REACHABLE : (lbl_step (ES.cont_thread S k))＊ st' st'')
-        (LBLS_EQ : lbls = opt_to_list lbl' ++ [lbl])
-        (RR : exists is_ex ord loc val, ⟪ LBL_LD : lbl = Aload is_ex ord loc val ⟫) :
-    exists k' e e' S', 
-      ⟪ ES_BSTEP_ : ESBasicStep.t_ (thread_lts (ES.cont_thread S k)) k k' st st' e e' S S' ⟫ /\
-      ⟪ LBL  : lbl  = S'.(ES.lab) e ⟫ /\
-      ⟪ LBL' : lbl' = option_map S'.(ES.lab) e' ⟫ /\
-      ⟪ CAJF : sim_add_jf S G sc TC TC' h k st e S' ⟫ /\
-      ⟪ EW' : S'.(ES.ew) ≡ ew ⟫ /\
-      ⟪ CO' : S'.(ES.co) ≡ co ⟫.
-  Proof. 
-    desf. 
-    assert (tc_coherent G sc TC') as TCCOH'. 
-    { eapply isim_trav_step_coherence; apply SRCC. }
-    assert ((K S) (k, existT Language.state (thread_lts (ES.cont_thread S k)) st)) as KK.
-    { edestruct cstate_q_cont; [apply SRCC|]. desf. }
-    assert (wf_thread_state (ES.cont_thread S k) st) as WFST.
-    { by apply SRCC. }
-    edestruct cert_rf_complete as [w RFwa]; 
-      eauto; try apply SRCC.
-    { assert 
-        (E0 G TC' (ES.cont_thread S k) (ThreadEvent (ES.cont_thread S k) st.(eindex)))
-        as E0_eindex.
-      { eapply ilbl_step_E0_eindex; eauto. 
-        all : by eapply SRCC. }
-      split; eauto.  
-      eapply same_lab_u2v_dom_is_r.
-      { apply same_lab_u2v_dom_comm.
-        eapply cuplab_cert; apply SRCC. }
-      split. 
-      { eapply dcertE; eauto; apply SRCC. }
-      unfold is_r.
-      erewrite steps_preserve_lab.  
-      { edestruct lbl_step_cases as [lbl [lbl'' HH]]; eauto.
-        destruct HH as [LBLS [HA | HB]].
-        all : apply opt_to_list_app_singl in LBLS.
-        { destruct HA as [_ [_ [LAB _]]].
-          rewrite LAB, upds. desf. }
-        destruct HB as [_ [_ [LAB LBLS']]].
-        rewrite LAB. unfold upd_opt. 
-        destruct lbl'' eqn:Heq. 
-        { rewrite updo, upds; desf.
-          intros HH. inversion HH. omega. }
-        exfalso. desf. }
-      { eapply wf_thread_state_steps; eauto.
-        eapply ilbl_steps_in_steps.
-        econstructor; econstructor; eauto. }
-      { by eapply ilbl_steps_in_steps. }
-      edestruct lbl_step_cases as [lbl [lbl'' HH]]; eauto.
-      destruct HH as [LBLS [HH | HH]].
-      all : apply opt_to_list_app_singl in LBLS.
-      all : destruct HH as [_ [ACTS _]].
-      all : apply ACTS; basic_solver. }
-    edestruct simrel_cert_basic_step as [k' [e [e' [S' BSTEP]]]]; eauto.
-    desf; do 4 eexists; splits; eauto.
-    econstructor; splits.  
-    { unfold is_r. by rewrite <- LBL. }
-    assert (cert_dom G TC (ES.cont_thread S k) st w) as HDOMw.
-    { eapply cert_rf_cert_dom; try apply SRCC; auto. 
-      { red. ins. eapply ES.init_tid_K; eauto. apply SRCC. }
-      unfold dom_rel. eexists.
-      apply seq_eqv_r; splits; eauto. }
-    assert 
-      ((h □₁ (cert_dom G TC (ES.cont_thread S k) st)) (h w)) 
-      as hHDOMhw. 
-    { unfolder; eexists; splits; eauto. }
-    exists (h w); splits; auto. 
-    2 : cdes ES_BSTEP_; desf; eauto. 
-    arewrite (e2a S' (h w) = w).  
-    { erewrite basic_step_e2a_eq_dom.
-      { eapply a2e_fix; eauto. apply SRCC. }
-      { apply SRCC. }
-      { econstructor; eauto. }
-      eapply a2e_img; eauto. apply SRCC. }
-    erewrite basic_step_e2a_e; eauto. 
-    all : apply SRCC.
-  Qed.
 
   (* Lemma weaken_sim_add_jf TC' h k k' e e' S'  *)
   (*       (st st' st'' : thread_st (ES.cont_thread S k)) *)
